src/impl/TLS13.Record.fsti
@@ -49,6 +49,7 @@ fn application_keys_match (st: record_state) (key: array U8.t) (alg: C.aead_alg)
           pts_to key 'key_bytes **
           pts_to iv 'iv_bytes **
           pure (ok ==>
+            's.R.alg == alg /\
             's.R.key == Some (C.logical_key alg 'key_bytes) /\
             's.R.static_iv == Some (Ghost.reveal 'iv_bytes))
 
@@ -82,7 +83,7 @@ fn install_keys
            pure (B.length 'key_bytes == 32 /\ B.length 'iv_bytes == 12 /\
                  C.aead_key_len alg == B.length key_spec /\
                  Seq.equal 'key_bytes (C.pad_key_32 key_spec))
-  ensures is_record_state st (R.install_keys 's epoch (Ghost.reveal key_spec) (Ghost.reveal 'iv_bytes)) **
+  ensures is_record_state st (R.install_keys 's epoch alg (Ghost.reveal key_spec) (Ghost.reveal 'iv_bytes)) **
           pts_to key 'key_bytes **
           pts_to iv 'iv_bytes
 
@@ -98,7 +99,7 @@ fn install_handshake_keys_runtime
            pure (B.length 'key_bytes == 32 /\ B.length 'iv_bytes == 12 /\
                  C.aead_key_len alg == B.length key_spec /\
                  Seq.equal 'key_bytes (C.pad_key_32 key_spec))
-  ensures is_record_state st (R.install_keys 's R.Handshake (Ghost.reveal key_spec) (Ghost.reveal 'iv_bytes)) **
+  ensures is_record_state st (R.install_keys 's R.Handshake alg (Ghost.reveal key_spec) (Ghost.reveal 'iv_bytes)) **
           pts_to key 'key_bytes **
           pts_to iv 'iv_bytes
 
@@ -114,7 +115,7 @@ fn install_application_keys_runtime
            pure (B.length 'key_bytes == 32 /\ B.length 'iv_bytes == 12 /\
                  C.aead_key_len alg == B.length key_spec /\
                  Seq.equal 'key_bytes (C.pad_key_32 key_spec))
-  ensures is_record_state st (R.install_keys 's R.Application (Ghost.reveal key_spec) (Ghost.reveal 'iv_bytes)) **
+  ensures is_record_state st (R.install_keys 's R.Application alg (Ghost.reveal key_spec) (Ghost.reveal 'iv_bytes)) **
           pts_to key 'key_bytes **
           pts_to iv 'iv_bytes
 
